prove basic configuration invariants

ironfleet/src/Dafny/Distributed/Protocol/ZooKeeper/PerformamceProof/BasicInvariants.dfy
@@ -11,7 +11,6 @@ include "../Follower.dfy"
 include "../Leader.dfy"
 include "../LearnerHandler.dfy"
 include "Definitions.dfy"
-// include "PerformancePredicates.dfy"
 
 
 /* This module contains invariants that have nothing to do with performance */
@@ -28,11 +27,17 @@ import opened ZooKeeper_Leader
 import opened ZooKeeper_LearnerHandler
 import opened Zookeeper_Performance_Definitions
 import opened ZooKeeper_TimestampedDistributedSystem
-// import opened Zookeeper_PerformancePredicates
+
+
+
+/*****************************************************************************************
+/                                   DSConfigInvariant                                    *
+*****************************************************************************************/
 
 
 /* config has same endpoints as tls.servers and each node's id is its index in config */
-predicate ConfigInvariant(config:Config, tls:TLS_State) {
+predicate DS_Config_Invariant(config:Config, tls:TLS_State) {
+    && |config| > 0
     && (forall ep :: ep in config <==> ep in tls.t_servers)
     && (forall ep | ep in tls.t_servers :: config == if tls.t_servers[ep].v.FollowerPeer? then tls.t_servers[ep].v.follower.config else tls.t_servers[ep].v.leader.config)
     && (forall i | 0 <= i < |config| :: 
@@ -40,25 +45,61 @@ predicate ConfigInvariant(config:Config, tls:TLS_State) {
     )
 }
 
-
-lemma lemma_Config_Invariant_Proof(config:Config, tlb:seq<TLS_State>, f:int)
+lemma lemma_DS_Config_Invariant_Proof(config:Config, tlb:seq<TLS_State>, f:int)
     requires SeqIsUnique(config);
     requires ValidTLSBehavior(config, tlb, f)
-    ensures forall i | 0 <= i < |tlb| :: ConfigInvariant(config, tlb[i])
+    ensures forall i | 0 <= i < |tlb| :: DS_Config_Invariant(config, tlb[i])
 {
-    assert ConfigInvariant(config, tlb[0]);
+    assert DS_Config_Invariant(config, tlb[0]);
     var i := 0;
     while i < |tlb| - 1 
         decreases |tlb| - i
         invariant 0 <= i < |tlb|
-        invariant forall k | 0 <= k <= i :: ConfigInvariant(config, tlb[k])
+        invariant forall k | 0 <= k <= i :: DS_Config_Invariant(config, tlb[k])
     {
         var tls, tls' := tlb[i], tlb[i+1];
         assert TLS_Next(tls, tls');
-        assert ConfigInvariant(config, tls');
+        assert DS_Config_Invariant(config, tls');
         i := i + 1;
     }
 }
 
 
+/*****************************************************************************************
+/                                   ZKConfigInvariant                                    *
+*****************************************************************************************/
+
+/* config[0] is the leader and everyone else are followers */
+predicate ZK_Config_Invariant(config:Config, tls:TLS_State) 
+    requires DS_Config_Invariant(config, tls)
+{   
+    // Only config[0] is the leader
+    && (forall i | 0 <= i < |config| :: if i == 0 then tls.t_servers[config[i]].v.LeaderPeer? else tls.t_servers[config[i]].v.FollowerPeer?)
+    // Every follower has 0 as the leader
+    && (forall ep | ep in tls.t_servers && tls.t_servers[ep].v.FollowerPeer? :: tls.t_servers[ep].v.follower.leader_id == 0)
+    // Each follower has a corresponding learner handler
+    && |tls.t_servers[config[0]].v.leader.handlers| == |config| - 1
+    && (forall follower_id | 1 <= follower_id < |config| :: tls.t_servers[config[0]].v.leader.handlers[follower_id-1].follower_id == follower_id)
+}
+
+
+lemma lemma_ZK_Config_Invariant_Proof(config:Config, tlb:seq<TLS_State>, f:int)
+    requires SeqIsUnique(config);
+    requires ValidTLSBehavior(config, tlb, f)
+    requires forall i | 0 <= i < |tlb| :: DS_Config_Invariant(config, tlb[i])
+    ensures forall i | 0 <= i < |tlb| :: ZK_Config_Invariant(config, tlb[i])
+{
+    assert ZK_Config_Invariant(config, tlb[0]);
+    var i := 0;
+    while i < |tlb| - 1 
+        decreases |tlb| - i
+        invariant 0 <= i < |tlb|
+        invariant forall k | 0 <= k <= i :: ZK_Config_Invariant(config, tlb[k])
+    {
+        var tls, tls' := tlb[i], tlb[i+1];
+        assert TLS_Next(tls, tls');
+        assert ZK_Config_Invariant(config, tls');
+        i := i + 1;
+    }
+}
 }
